LeanYjs/ItemSet.lean
@@ -10,8 +10,8 @@ def ItemSet := Set (YjsPtr A)
 structure IsClosedItemSet {A} (P : YjsPtr A -> Prop) : Prop where
   baseFirst : P YjsPtr.first
   baseLast : P YjsPtr.last
-  closedLeft : (∀ (o : YjsPtr A) r id c d, P (YjsItem.item o r id c d) -> P o)
-  closedRight : (∀ o (r : YjsPtr A) id c d, P (YjsItem.item o r id c d) -> P r)
+  closedLeft : (∀ (o : YjsPtr A) r id c d, P (YjsItem.mk o r id c d) -> P o)
+  closedRight : (∀ o (r : YjsPtr A) id c d, P (YjsItem.mk o r id c d) -> P r)
 
 theorem IsClosedItemSet.eq_set {A} (P Q : YjsPtr A -> Prop) :
   IsClosedItemSet P ->
