LeanYjs/Algorithm/Delete/Basic.lean
@@ -1,0 +1,9 @@
+import LeanYjs.Item
+
+def deleteById (arr : Array (YjsItem A)) (id : YjsId) : Array (YjsItem A) :=
+  -- Mark the item with the given id as deleted
+  arr.map (fun item =>
+    if item.id = id then
+      YjsItem.mk item.origin item.rightOrigin item.id item.content true
+    else
+      item)
