LeanYjs/Algorithm/YString.lean
@@ -1,6 +1,8 @@
 import LeanYjs.Item
 import LeanYjs.ClientId
-import LeanYjs.Algorithm.Integrate
+import LeanYjs.Algorithm.Basic
+import LeanYjs.Algorithm.Insert.Basic
+import LeanYjs.Algorithm.Delete.Basic
 
 abbrev Item := YjsItem Char
 structure YString : Type where
@@ -15,26 +17,36 @@ def extGetElemExcept (arr : Array (YjsItem A)) (idx : Int) : Except IntegrateErr
     Except.ok YjsPtr.last
   else
     if idx < 0 || idx >= arr.size then
-      Except.error IntegrateError.notFound
+      Except.error IntegrateError.error
     else
       match arr[idx.toNat]? with
       | some item => return item
-      | none => Except.error IntegrateError.notFound
+      | none => Except.error IntegrateError.error
 
 def nextId (currentId : YjsId) : YjsId :=
   YjsId.mk currentId.clientId (currentId.clock + 1)
 
 def YString.insert (s : YString) (i : Nat) (c : Char) : StateT YjsId (Except IntegrateError) YString := do
   if i > s.contents.size then
-    throw $ IntegrateError.notFound
+    throw $ IntegrateError.error
   let arr : Array Item := s.contents
   let origin <- extGetElemExcept arr (Int.ofNat i - 1)
   let rightOrigin <- extGetElemExcept arr (Int.ofNat i)
   let id := nextId (← StateT.get)
-  let newItem : Item := YjsItem.item origin rightOrigin id c false
+  let newItem : Item := YjsItem.mk origin rightOrigin id c false
   let arr <- integrate newItem s.contents
   pure { contents := arr }
 
+def YString.delete (s : YString) (i : Nat) : Except IntegrateError YString :=
+  if i >= s.contents.size then
+    Except.error IntegrateError.error
+  else
+    let arr := s.contents
+    match arr[i]? with
+    | some item => do
+      let newArr := deleteById s.contents item.id
+      Except.ok { contents := newArr }
+    | none => Except.error IntegrateError.error
+
 def YString.toString (s : YString) : String :=
   String.ofList $ (s.contents.map (fun item => item.content)).toList
-  
